Clean.

core/Metamodel.v
@@ -3,8 +3,8 @@
 
 Record Metamodel :=
 {
-    ElementType: Type;
-    LinkType: Type;
+    ElementType: Set;
+    LinkType: Set;
     
     elements_eqdec: ElementType -> ElementType -> bool; (* FIXME : no semantics with respect to equality *)
     links_eqdec: LinkType -> LinkType -> bool; 
