transformations/Class2Relational/theorems/C2R_monotonicity.v
@@ -32,7 +32,8 @@ Proof.
   intros sm1 sm2 INC a IN.
 
   (* (1) *)
-  Tactics.chain_destruct_in_modelElements_execute IN.
+  destruct (Tactics.destruct_in_modelElements_execute_lem IN) 
+    as (r & sp & n & ope & IN_E & IN_RULE & MATCH_GUARD & IN_IT & IN_OP & IN'). 
 
   (* (2)  *)
   Tactics.progress_in_In_rules IN_RULE ; [ | ] ;
@@ -46,7 +47,7 @@ Proof.
 
   
   (* (5) *)
-  Tactics.exploit_evaloutpat IN ;
+  Tactics.exploit_evaloutpat IN' ;
   
   (* (6) *)
   clear IN_IT ;
