transformations/Class2Relational/theorems/Table_name_uniqueness.v
@@ -47,7 +47,8 @@ Proof.
   
     
   (* (1) *)
-  Tactics.chain_destruct_in_modelElements_execute IN1.
+  destruct (Tactics.destruct_in_modelElements_execute_lem IN1) 
+    as (r & sp & n & ope & IN_E & IN_RULE & MATCH_GUARD & IN_IT & IN_OP & IN1'). 
 
   (* (2) *)
   Tactics.progress_in_In_rules IN_RULE ; [ |  ];
@@ -59,7 +60,7 @@ Proof.
   Tactics.exploit_evalGuard MATCH_GUARD ;
 
   (* (5.E) *)
-  Tactics.exploit_evaloutpat IN1 ; subst ; [] ;
+  Tactics.exploit_evaloutpat IN1' ; subst ; [] ;
 
   (* (6) *)
   Tactics.exploit_in_it IN_IT ;
@@ -69,7 +70,8 @@ Proof.
 
 
   (* (1) *)
-  Tactics.chain_destruct_in_modelElements_execute IN2.
+  destruct (Tactics.destruct_in_modelElements_execute_lem IN2) 
+    as (r & sp & n & ope & IN_E2 & IN_RULE & MATCH_GUARD & IN_IT & IN_OP & IN2'). 
 
   (* (2) *)
   Tactics.progress_in_In_rules IN_RULE ; [ |  ];
@@ -82,7 +84,7 @@ Proof.
   Tactics.exploit_evalGuard MATCH_GUARD ;
   
   (* (5.E) *) 
-  Tactics.exploit_evaloutpat IN2 ;
+  Tactics.exploit_evaloutpat IN2' ;
 
   (* (6) *)
   (* useless here *)
