transformations/Class2Relational_TUPLE_SP/C2RTactics.v
@@ -111,113 +111,6 @@ Ltac unify_column_attribute_tac H :=
           apply unify_column_attribute_lem in H ; destruct H as [H2 H] ; subst c
   end.
 
-(*
-Ltac unify_all :=
-  match goal with
-    [ H : In (ColumnElement _) (instantiatePattern Class2Relational _ [AttributeElement _]) |- _ ] =>
-      unify_column_attribute_tac H
-
-   | [ H : In (TableElement _) (instantiatePattern Class2Relational _ [ClassElement _]) |- _ ] => unify_table_class_tac H
-  end.
-
-Lemma make1 sm e :
-  ConcreteExpressions.makeEmptyGuard [Class_K] sm [e] = true ->
-  exists v, e = ClassElement v. 
-Proof.
-  destruct e ; compute ; intro M ; [ eauto | discriminate].
-Qed.
-
-Lemma make1_alt sm e :
-  ConcreteExpressions.makeEmptyGuard [Class_K] sm e = true ->
-  exists v, e = [ClassElement v]. 
-Proof.
-  destruct e ; intro H. 
-  + discriminate H.  
-  + destruct e.
-    - apply make1 in H. destruct H ; subst ; eauto.
-    - compute in  H. 
-      destruct s ; discriminate .
-Qed.
-
-Lemma make2 sm e:
-  ConcreteExpressions.makeGuard [Attribute_K]
-    (fun (_ : TransformationConfiguration.SourceModel)
-         (a : Attribute_t) => negb (derived a)) sm 
-    [e] = true -> exists v, (e = AttributeElement v /\ v.(derived) = false).
-Proof.
-  destruct e ; [ discriminate | ] ; compute.
-  destruct a.
-  destruct derived ; [ discriminate | ].
-  eauto.
-Qed.
-
-Lemma make2_alt sm e:
-  ConcreteExpressions.makeGuard [Attribute_K]
-    (fun (_ : TransformationConfiguration.SourceModel)
-         (a : Attribute_t) => negb (derived a)) sm 
-    e = true -> exists v, (e = [AttributeElement v] /\ v.(derived) = false).
-Proof.
-  destruct e ; intro.
-  + discriminate H.
-  + destruct e.
-  - apply make2 in H.
-    destruct H as (? & (? & ?)) ; subst.
-    eauto.
-  - compute in H. 
-    destruct s ; discriminate H.
-Qed.
-
-
-
-Ltac deduce_element_kind_from_guard :=
-  let H2 := fresh "D" in
-  let a := fresh "a" in
-  match goal with 
-    [ H :ConcreteExpressions.makeEmptyGuard [Class_K] _ [?e] = true |- _ ] =>
-      apply make1 in H ; destruct H ; subst e
-
-    | [ H :ConcreteExpressions.makeEmptyGuard [Class_K] _ ?e = true |- _ ] =>
-      apply make1_alt in H ; destruct H ; subst e
-
-
-  | [ H :ConcreteExpressions.makeGuard [Attribute_K]
-    (fun _ atr => negb (derived atr)) _ 
-    [?e] = true |- _ ] =>
-      apply make2 in H ; destruct H as (a & (H & H2)) ; 
-      first[ subst e (* if e was a variable *) 
-             | Tactics.inj H (* if e was not a variable *) ]
-
-  | [ H :ConcreteExpressions.makeGuard [Attribute_K]
-    (fun _ atr => negb (derived atr)) _ 
-    ?e = true |- _ ] =>
-      apply make2_alt in H ; destruct H as (a & (H & H2)) ; 
-      (*first[*) subst e (* if e was a variable *) 
-             (*| Tactics.inj H (* if e was not a variable *) ]*)
-end.
-
-
-(** ** Size of patterns *)
-
-Lemma one_to_one : 
-  Tactics.singleton_transformation_a _ Class2Relational.
-Proof.
-  apply Tactics.singleton_transformation_parse.
-  unfold Class2Relational' ; unfold Tactics.singleton_transformation_a ; simpl ; repeat constructor.
-Qed.
-
-Hint Resolve one_to_one : singleton_rules.
-
-
-(** ** Destructors *)
-
-Ltac destruct_In_two :=
-  match goal with 
-    [ H : In ?X Class2Relational.(Syntax.rules) |- _ ] => 
-      simpl in H ; 
-      unfold In in H ; (* force it because simpl In can be disabled by Arguments In: simpl never. *)
-
-      repeat destruct_or H ; [ | | contradiction H] ; subst X
-  end.*)
 
 
 (** *** Utilities on [allTuples] *)
@@ -233,7 +126,7 @@ Proof.
   auto.
 Qed. 
 
-(** Specific tactics for this transformation. *)
+(** * Specific tactics for this transformation. *)
 Ltac exploit_guard H := 
   match type of H with
     andb (negb _) (is_option_eq _ _ _) = true =>
