transformations/Class2Relational_TUPLE_SP/theorems/Column_name_uniqueness.v
@@ -47,7 +47,9 @@ Proof.
 
 
     (* (1) *)
-    Tactics.chain_destruct_in_modelElements_execute IN1.
+    destruct (Tactics.destruct_in_modelElements_execute_lem IN1) 
+    as (r & sp & n & ope & IN_E & IN_RULE & MATCH_GUARD & IN_IT & IN_OP & IN1').    
+
    
     (* (2) *)
     Tactics.progress_in_In_rules IN_RULE ; [ | ] ; 
@@ -60,7 +62,7 @@ Proof.
     Tactics.exploit_evalGuard MATCH_GUARD ;
 
     (* (5.E) *)
-    Tactics.exploit_evaloutpat IN1 ; 
+    Tactics.exploit_evaloutpat IN1' ; 
 
     (* (6) *)
     clear IN_IT ;
@@ -71,7 +73,9 @@ Proof.
 
 
     (* (1) *)
-    Tactics.chain_destruct_in_modelElements_execute IN2.
+    destruct (Tactics.destruct_in_modelElements_execute_lem IN2) 
+      as (r & sp & n2 & ope & IN_E2 & IN_RULE & MATCH_GUARD2 & IN_IT & IN_OP & IN2').    
+
     
     (* (2) *)
     Tactics.progress_in_In_rules IN_RULE ; [ | ]; 
@@ -81,16 +85,16 @@ Proof.
 
     (* (4) *)
     (* not useful here *)
-    Tactics.exploit_evalGuard MATCH_GUARD0 ;
+    Tactics.exploit_evalGuard MATCH_GUARD2 ;
     
     (* (5) *)
-    Tactics.exploit_evaloutpat IN2 ; 
+    Tactics.exploit_evaloutpat IN2' ; 
 
     (* (6) *)
     clear IN_IT ;
 
     (* (7) *)
-    exploit_in_allTuples IN_E1 ; [].
+    exploit_in_allTuples IN_E2 ; [].
         
     simpl.
 
